\chapter{Partial Differentiation}

\section{The Partial Derivative}

\begin{equation*}
    \frac{\partial f}{\partial x} = \lim_{\Delta x \to 0}\frac{f(x + \Delta x, y) - f(x, y)}{\Delta x}
\end{equation*}

\begin{equation*}
    \frac{\partial f}{\partial y} = \lim_{\Delta y \to 0}\frac{f(x, y + \Delta y) - f(x, y)}{\Delta y}
\end{equation*}

\[\frac{\partial}{\partial x}\left(\frac{\partial f}{\partial x}\right) = \frac{\partial^{2}f}{\partial x ^{2}} \qquad \frac{\partial}{\partial y}\left(\frac{\partial f}{\partial y}\right) = \frac{\partial^{2}f}{\partial y ^{2}}\]

\begin{equation*}
    \frac{\partial^{2}f}{\partial x \partial y} = \frac{\partial^{2}f}{\partial y \partial x}
\end{equation*}

\section{The Total Differential}

\begin{equation*}
    \Delta f \approx \frac{\partial f(x, y)}{\partial x}\Delta x + \frac{\partial f(x, y)}{\partial y}\Delta y
\end{equation*}

\begin{equation*}
    df = \frac{\partial f(x, y)}{\partial x}dx + \frac{\partial f(x, y)}{\partial y}dy
\end{equation*}

\begin{equation*}
    df = \sum_{i}^{n}\frac{\partial f}{\partial x_{i}}dx_{i}
\end{equation*}

\begin{equation*}
    \frac{df}{dx_{1}} = \sum_{i}^{n}\left(\frac{\partial f}{\partial x_{i}}\right)\frac{dx_{i}}{dx_{1}}
\end{equation*}

\section{Exact Differentials}

\begin{equation*}
    df = A(x, y)dx + B(x, y)dy
\end{equation*}

\begin{equation*}
    \frac{\partial f}{\partial x} = A(x, y), \qquad \frac{\partial f}{\partial y} = B(x, y)
\end{equation*}

\begin{equation*}
    \frac{\partial A}{\partial x} = \frac{\partial B}{\partial x}
\end{equation*}

\section{Change of Variables}

\begin{equation*}
    x_i = x_i(u_1, u_2, ..., u_m)
\end{equation*}

\begin{equation*}
    \frac{\partial f}{\partial x_j} = 
    \sum_{i=1}^{n}\frac{\partial f}{\partial x_i}
    \frac{\partial x_i}{\partial x_j}
\end{equation*}

\section{Maxima and Minima}

\begin{equation*}
    \frac{\partial f}{\partial x} = 0, \qquad \frac{\partial f}{\partial y} = 0
\end{equation*}

\section{Lagrange Multipliers}

\begin{equation*}
    df = \frac{\partial f}{\partial x}dx + \frac{\partial f}{\partial y}dy = 0
\end{equation*}

\begin{equation*}
    dg = \frac{\partial g}{\partial x}dx + \frac{\partial g}{\partial y}dy = 0
\end{equation*}

\begin{equation*}
    \frac{\partial f}{\partial x} = \lambda\frac{\partial g}{\partial x}
\end{equation*}

\begin{equation*}
    \frac{\partial f}{\partial y} = \lambda\frac{\partial g}{\partial y}
\end{equation*}

\section{Leibnitz' Rule}

\begin{equation*}
    F(x,t) = \int f(x,t)dt
\end{equation*}

\begin{equation*}
    \frac{\partial F(x,t)}{\partial x} = f(x,t)
\end{equation*}

\begin{equation*}
    \frac{\partial^{2}F(x,t)}{\partial t \partial x} = \frac{\partial^{2}F(x,t)}{\partial x \partial t}
\end{equation*}

\begin{equation*}
    \frac{\partial}{\partial t}\left[\frac{\partial F(x,t)}{\partial x}\right] =
    \frac{\partial}{\partial x}\left[\frac{\partial F(x,t)}{\partial t}\right] =
    \frac{\partial f(x,t)}{\partial x}
\end{equation*}

\begin{equation*}
    \frac{\partial F(x,t)}{\partial x} = \int \frac{\partial f(x,t)}{\partial x} dt
\end{equation*}

\begin{align*}
    I(x) &= \int_{t=v}^{t=u}f(x,t)dt\\
    &= F(x,v) - F(x,u)
\end{align*}

\begin{align*}
    \frac{dI(x)}{dx} &= \frac{\partial F(x,v)}{\partial x} - \frac{\partial F(x,u)}{\partial x}\\
    &= \int^{v} \frac{\partial f(x,t)}{\partial x}dt - \int^{u} \frac{\partial f(x,t)}{\partial x}dt\\
    &= \int_{u}^{v} \frac{\partial f(x,t)}{\partial x}dt
\end{align*}

\begin{align*}
    I(x) &= \int_{t=v(x)}^{t=u(x)}f(x,t)dt\\
    &= F(x,v(x)) - F(x,u(x))
\end{align*}