\chapter{Series}

\section{Series}
\section{Convergence Tests}
\section{Power Series}

\section{Taylor Series}

\begin{equation*}
    f(x) = a_0 + a_1 x + a_2 x^2 + a_3 x^3 + \dots = \sum_{n}^{\infty}a_n x^n
\end{equation*}

\begin{equation*}
    f'(x) = a_1 + 2a_2 x + 3a_3 x^2 + \dots = \sum_{n}^{\infty}n a_n x^{n-1}
\end{equation*}

\begin{equation*}
    f''(x) = \sum_{n}^{\infty} n(n-1) a_n x^{n-2}
\end{equation*}

\begin{equation*}
    f(x) = f(a) + (x-a)f'(a) + \frac{(x-a)^2}{2!}f''(a) + 
\end{equation*}

\begin{equation*}
    \sin(x) = x - \frac{x^{3}}{3!} + \frac{x^{5}}{5!} - \frac{x^{7}}{7!} + \dots
\end{equation*}

\begin{equation*}
    \cos(x) = 1 - \frac{x^{2}}{2!} + \frac{x^{4}}{4!} - \frac{x^{6}}{6!} + \dots
\end{equation*}

\begin{equation*}
    e^{x} = 1 + \frac{x^{2}}{2!} + \frac{x^{3}}{3!} + \frac{x^{4}}{4!} + \dots
\end{equation*}

\section{Lâ€™Hopital's Rule}